\section{Appendix}
\label{sec:appendix}
\subsection{Bayes Model explanation}
\label{app:bayes_model}
We identified Bayes Model in equation (\ref{eq:bayes_model}) as such
\begin{align}
\phi_{\beta} & = \underset{c \,\in\, Y}{argmin} \; \mathbb{E}_{Y|X=x}\{L(Y,c) \} \notag\\
			 & = \underset{c \,\in\, Y}{argmin} \; P(Y \neq c \,| X = x) \notag\\
			 & = \underset{c \,\in\, Y}{argmax} \; P(Y = c \,| X = x)\notag
\end{align}

\subsection{Bias-variance decomposition of Squared Loss Function}
\label{app:bias_var_decomp}
We derived the result in equation (\ref{eq:decomp_squared_loss}) as follows;
\begin{align}
\boldsymbol{Err}(T_{D, \theta}(x)) & = \mathbb{E}_{Y|X=x}\{(Y-T_{D,\theta}(x))^2\} \notag \\
							  & = \mathbb{E}_{Y|X=x}\{(Y -\phi_{\beta}(x) +\phi_{\beta}(x) -T_{D,\theta}(x))^2\} \notag \\
							  & = \mathbb{E}_{Y|X=x}\{(Y-\phi_{\beta}(x))^2\} + \mathbb{E}_{Y|X=x}\{(\phi_{\beta}(x)-T_{D,\theta}(x))^2\} \notag \\
							  &	\: + \underbrace{\mathbb{E}_{Y|X=x}\{2(Y-\phi_{\beta}(x))(\phi_{\beta}(x)-T_{D,\theta}(x))\}}_\text{$=0$ \ since $ \mathbb{E}_{Y|X=x}(Y-\phi_{\beta}(x)) = 0$ from \ref{eq:bayes_eq_y}}  \notag \\
							  & = \underbrace{\mathbb{E}_{Y|X=x}\{(Y-\phi_{\beta}(x))^2\}}_\text{from \ref{eq:err_bayes} equals to $\boldsymbol{Err}(\phi_{\beta}(x))$} + \mathbb{E}_{Y|X=x}\{(\phi_{\beta}(x)-T_{D,\theta}(x))^2\}  \notag \\
							  & = \boldsymbol{Err}(\phi_{\beta}(x)) + (\phi_{\beta}(x)-T_{D,\theta}(x))^2\notag
\end{align}

